case_study/RiscvPmp/Model.v
@@ -175,9 +175,9 @@ Module RiscvPmpModel.
         | Some (lo, hi) =>
             if hi <? lo
             then PMP_NoMatch
-            else if (a<? lo) || (hi <? a)
+            else if (a <? lo) || (hi <=? a)
                  then PMP_NoMatch
-                 else if (lo <=? a) && (a <=? hi)
+                 else if (lo <=? a) && (a <? hi)
                       then PMP_Match
                       else PMP_PartialMatch
         | None          => PMP_NoMatch
@@ -209,18 +209,20 @@ Module RiscvPmpModel.
       Definition pmp_match_entry (a : Addr) (m : Privilege) (cfg : Pmpcfg_ent) (lo hi : Xlenbits) : PmpMatch * Permission :=
         let rng := pmp_addr_range cfg hi lo in
         match pmp_match_addr a rng with
-        | PMP_NoMatch      => (PMP_Continue , O)
+        | PMP_NoMatch      => (PMP_Continue, O)
         | PMP_PartialMatch => (PMP_Fail, O)
         | PMP_Match        => (PMP_Success, pmp_permission m cfg)
         end.
 
-      (* TODO: if nothing matches we should check m and give full perm if m is M-mode *)
       Fixpoint pmp_check (a : Addr) (entries : list PmpEntryCfg) (prev : Addr) (m : Privilege) : option Permission :=
         match entries with
-        | [] => None
+        | [] => match m with
+                | Machine => Some RW
+                | User    => None
+                end
         | (cfg , addr) :: entries =>
             match pmp_match_entry a m cfg prev addr with
-            | (PMP_Success , p) => Some p
+            | (PMP_Success, p)  => Some p
             | (PMP_Fail, _)     => None
             | (PMP_Continue, _) => pmp_check a entries addr m
             end
@@ -232,21 +234,40 @@ Module RiscvPmpModel.
       Definition check_access (a : Addr) (entries : list PmpEntryCfg) (m : Privilege) : option Permission :=
         pmp_check a entries 0 m.
 
+      Lemma pmp_match_entry_TOR_within_bounds :
+        forall (a : Addr) (m : Privilege) (cfg : Pmpcfg_ent) (lo hi : Xlenbits),
+          lo <= a ∧ a < hi ->
+          A cfg = TOR ->
+          pmp_match_entry a m cfg lo hi = (PMP_Success, pmp_permission m cfg).
+      Proof.
+        intros a m [] lo hi [Hlo Hhi] [= ->].
+        unfold pmp_match_entry.
+        simpl.
+        assert (H: lo <= hi) by (eapply Z.le_trans with (m := a); try assumption;
+                                 try (apply Z.lt_le_incl; assumption)).
+        apply Z.ltb_ge in H; apply Z.ltb_ge in Hlo; apply Z.ltb_lt in Hhi.
+        rewrite H Hhi Hlo; simpl.
+        rewrite ?Z.leb_antisym Hlo Hhi; simpl; auto.
+      Qed.
+
       (* TODO: add perm_access predicate *)
       (* pmp_addr_access(?entries, ?mode) 
          ∀ a ∈ Mem, p : Perm . check_access(a, entries, mode) = Some p -> 
                                ∃ w . a ↦ w ∗ perm_access(a, p) *)
-      Definition interp_pmp_addr_access `{sailRegGS Σ} `{invGS Σ} {mG : memGS Σ} (entries : list PmpEntryCfg) (m : Privilege) : iProp Σ :=
-        [∗ list] a ∈ liveAddrs,
+      Definition interp_pmp_addr_access `{sailRegGS Σ} `{invGS Σ} {mG : memGS Σ} (addrs : list Addr) (entries : list PmpEntryCfg) (m : Privilege) : iProp Σ :=
+        [∗ list] a ∈ addrs,
           (⌜∃ p, check_access a entries m = Some p⌝ -∗
             (∃ w, mapsto (hG := mc_ghGS (mcMemGS := mG)) a (DfracOwn 1) w))%I.
 
+      Definition interp_ptsto `{sailRegGS Σ} `{invGS Σ} {mG : memGS Σ} (addr : Addr) (w : Word) : iProp Σ :=
+        mapsto (hG := mc_ghGS (mcMemGS := mG)) addr (DfracOwn 1) w. 
+
       Definition luser_inst `{sailRegGS Σ} `{invGS Σ} (mG : memGS Σ) (p : Predicate) : Env Val (𝑯_Ty p) -> iProp Σ :=
         match p return Env Val (𝑯_Ty p) -> iProp Σ with
-        | pmp_entries     => fun ts => interp_pmp_entries (env.head ts)
-        | pmp_addr_access => fun ts => interp_pmp_addr_access (mG := mG) (env.head (env.tail ts)) (env.head ts)
-        | gprs            => fun _  => interp_gprs
-        | ptsto           => fun _  => True%I (* TODO: interp_ptst *)
+        | pmp_entries       => fun ts => interp_pmp_entries (env.head ts)
+        | pmp_addr_access   => fun ts => interp_pmp_addr_access (mG := mG) liveAddrs (env.head (env.tail ts)) (env.head ts)
+        | gprs              => fun _  => interp_gprs
+        | ptsto             => fun ts => interp_ptsto (mG := mG) (env.head (env.tail ts)) (env.head ts)
         end.
 
     Definition lduplicate_inst `{sailRegGS Σ} `{invGS Σ} (mG : memGS Σ) :
@@ -319,22 +340,211 @@ Module RiscvPmpModel.
     Proof.
       intros ι; destruct_syminstance ι; cbn.
       unfold RiscvPmpIrisHeapKit.interp_pmp_entries.
-      iIntros "[%cfg0 [%addr0 [%cfg1 [%addr1 [Hcfg0 [Haddr0 [Hcfg1 [Haddr1 %H]]]]]]]]".
-      destruct H as [H _].
-      destruct entries; try discriminate.
-      destruct v as [cfg0' addr0'].
-      destruct entries; try discriminate.
-      destruct v as [cfg1' addr1'].
+      iIntros "[%cfg0 [%addr0 [%cfg1 [%addr1 [Hcfg0 [Haddr0 [Hcfg1 [Haddr1 [%H _]]]]]]]]]".
+      destruct entries as [|[cfg0' addr0']]; try discriminate.
+      destruct entries as [|[cfg1' addr1']]; try discriminate.
       destruct entries; try discriminate.
       inversion H; subst.
       iAccu.
     Qed.
+
+    Lemma andb_leb_iff : forall (a b c d : Z),
+        (a <=? b)%Z && (c <=? d)%Z = true <-> (a <= b)%Z /\ (c <= d)%Z.
+    Proof.
+      intros; split; intro H.
+      - apply andb_prop in H as [H1 H2].
+        apply Zle_bool_imp_le in H1.
+        apply Zle_bool_imp_le in H2.
+        apply (conj H1 H2).
+      - destruct H as [H1 H2].
+        apply Zle_imp_le_bool in H1.
+        apply Zle_imp_le_bool in H2.
+        apply andb_true_intro.
+        apply (conj H1 H2).
+    Qed.
+
+    Lemma andb_leb_ltb_iff : forall (a b c d : Z),
+        (a <=? b)%Z && (c <? d)%Z = true <-> (a <= b)%Z /\ (c < d)%Z.
+    Proof.
+      intros; split; intro H.
+      - apply andb_prop in H as [H1 H2].
+        apply Zle_bool_imp_le in H1.
+        apply Z.ltb_lt in H2.
+        apply (conj H1 H2).
+      - destruct H as [H1 H2].
+        apply Zle_imp_le_bool in H1.
+        apply Z.ltb_lt in H2.
+        apply andb_true_intro.
+        apply (conj H1 H2).
+    Qed.
+
+    Lemma pmpcfg_ent_eqb_iff : forall cfg cfg',
+      pmpcfg_ent_eqb cfg cfg' = true <-> cfg = cfg'.
+    Proof.
+      intros [[] [] [] [] []] [[] [] [] [] []]; split;
+        intro H; simpl in H; subst; auto; discriminate.
+    Qed.
+
+    Lemma within_cfg_pmp_match_entry (a : Addr) (cfg : Pmpcfg_ent) (prev_addr addr : Addr) (p : Privilege) :
+        Within_cfg a cfg prev_addr addr ->
+        RiscvPmpIrisHeapKit.pmp_match_entry a p cfg prev_addr addr = (PMP_Success, RiscvPmpIrisHeapKit.pmp_permission p cfg).
+    Proof.
+      destruct cfg as [? [] ? ? ?]; intro H;
+        unfold Within_cfg, decide_within_cfg in H; simpl in H; try discriminate.
+      unfold RiscvPmpIrisHeapKit.pmp_match_entry,
+        RiscvPmpIrisHeapKit.pmp_match_addr; simpl.
+      apply andb_leb_ltb_iff in H as [Hprev Haddr].
+      assert (Hprevaddr: (prev_addr <= addr)%Z)
+        by (eapply Z.le_trans with (m := a); try assumption;
+            try (apply Z.lt_le_incl; assumption)).
+      simpl; rewrite ?Z.leb_antisym.
+      apply Z.ltb_ge in Hprevaddr as ->.
+      apply Z.ltb_ge in Hprev as ->.
+      apply Z.ltb_lt in Haddr as ->.
+      auto.
+    Qed.
+
+    Lemma extract_pmp_ptsto_sound :
+      ValidLemma RiscvPmpSpecification.lemma_extract_pmp_ptsto.
+    Proof.
+      intros ι; destruct_syminstance ι; cbn.
+      iIntros "[%cfg0 [%addr0 [%cfg1 [%addr1 [[%H _] [Hpmp_addr_access [[[%HNot _] [%Hp _]]|[[%HIn _] [[%HPrev _] [%HWithin _]]]]]]]]]]".
+      { unfold RiscvPmpIrisHeapKit.interp_pmp_addr_access.
+        assert (Hin: paddr ∈ RiscvPmpIrisHeapKit.liveAddrs) by admit.
+        iInduction RiscvPmpIrisHeapKit.liveAddrs as [|x xs] "IH".
+        - apply elem_of_nil in Hin; contradiction.
+        - apply elem_of_cons in Hin as [Heq|Hin].
+          + rewrite big_opL_cons.
+            iDestruct "Hpmp_addr_access" as "[Haccess _]".
+            unfold RiscvPmpIrisHeapKit.interp_ptsto; subst.
+            iApply "Haccess".
+            iPureIntro.
+            rename x into paddr.
+            eexists.
+            unfold Not_within_cfg, decide_not_within_cfg in HNot.
+            apply orb_prop in HNot as [HNot|HNot].
+            * apply andb_prop in HNot as [Hcfg0 Hcfg1].
+              destruct cfg0 as [? [] ? ? ?];
+                destruct cfg1 as [? [] ? ? ?];
+                simpl in *; auto.
+              (* TODO: the following doesn't seem the right way to do things =) *)
+              rewrite PmpAddrMatchType_eqb_equation_3 in Hcfg1; discriminate.
+              rewrite PmpAddrMatchType_eqb_equation_3 in Hcfg0; discriminate.
+              rewrite PmpAddrMatchType_eqb_equation_3 in Hcfg1; discriminate.
+            * unfold RiscvPmpIrisHeapKit.check_access,
+                RiscvPmpIrisHeapKit.pmp_check,
+                RiscvPmpIrisHeapKit.pmp_match_entry,
+                RiscvPmpIrisHeapKit.pmp_match_addr,
+                RiscvPmpIrisHeapKit.pmp_addr_range.
+              apply andb_prop in HNot as [HNot Haddr1].
+              apply andb_prop in HNot as [H0 Haddr0].
+              destruct cfg0 as [? [] ? ? ?]; simpl;
+                destruct cfg1 as [? [] ? ? ?]; simpl;
+                auto.
+              (* TODO: very bruteforce atm, clean this up *)
+              destruct (addr1 <? addr0)%Z; auto.
+              rewrite (Z.leb_antisym paddr addr1).
+              apply Zle_bool_imp_le in Haddr1.
+              apply Z.ltb_ge in Haddr1 as [= ->]; simpl.
+              rewrite orb_true_r; auto.
+              destruct (addr0 <? 0)%Z; auto.
+              rewrite (Z.leb_antisym paddr addr0).
+              apply Zle_bool_imp_le in Haddr0.
+              apply Z.ltb_ge in Haddr0 as [= ->]; simpl.
+              rewrite orb_true_r; auto.
+              destruct (addr0 <? 0)%Z; auto.
+              destruct (addr1 <? addr0)%Z; auto.
+              rewrite (Z.leb_antisym paddr addr1).
+              apply Zle_bool_imp_le in Haddr1.
+              apply Z.ltb_ge in Haddr1 as [= ->]; simpl.
+              rewrite orb_true_r; auto.
+              destruct (addr0 <? 0)%Z; auto.
+              rewrite (Z.leb_antisym paddr addr0).
+              apply Zle_bool_imp_le in Haddr0.
+              apply Z.ltb_ge in Haddr0 as [= ->]; simpl.
+              rewrite orb_true_r; auto.
+              rewrite (Z.leb_antisym paddr addr1).
+              apply Zle_bool_imp_le in Haddr1.
+              apply Z.ltb_ge in Haddr1 as [= ->]; simpl.
+              destruct (addr1 <? addr0)%Z; auto.
+              rewrite (Z.leb_antisym paddr addr0).
+              apply Zle_bool_imp_le in Haddr0.
+              apply Z.ltb_ge in Haddr0 as [= ->]; simpl.
+              rewrite orb_true_r; auto.
+              rewrite (Z.leb_antisym paddr addr1).
+              apply Zle_bool_imp_le in Haddr1.
+              apply Z.ltb_ge in Haddr1 as [= ->]; simpl.
+              destruct (addr1 <? addr0)%Z; auto.
+          + rewrite big_opL_cons.
+            iDestruct "Hpmp_addr_access" as "[_ H]".
+            iApply "IH"; try done.
+      }
+      { unfold RiscvPmpIrisHeapKit.interp_pmp_addr_access.
+        assert (Hin: paddr ∈ RiscvPmpIrisHeapKit.liveAddrs) by admit.
+        iInduction RiscvPmpIrisHeapKit.liveAddrs as [|x xs] "IH".
+        - apply elem_of_nil in Hin; contradiction.
+        - apply elem_of_cons in Hin as [Heq|Hin].
+          + destruct cfgidx; subst; simpl in *.
+            * iDestruct "Hpmp_addr_access" as "[H _]".
+              iClear "IH".
+              iApply "H".
+              iPureIntro.
+              exists (RiscvPmpIrisHeapKit.pmp_permission p cfg).
+              unfold RiscvPmpIrisHeapKit.check_access,
+                RiscvPmpIrisHeapKit.pmp_check.
+              unfold In_entries in HIn.
+              simpl in HIn.
+              apply andb_true_iff in HIn as [Heq Ha].
+              apply Z.eqb_eq in Ha; subst.
+              apply pmpcfg_ent_eqb_iff in Heq as [= ->].
+              unfold Prev_addr in HPrev.
+              simpl in HPrev.
+              apply Z.eqb_eq in HPrev as [= ->].
+              rewrite within_cfg_pmp_match_entry; try assumption.
+              auto.
+            * iDestruct "Hpmp_addr_access" as "[H _]".
+              iClear "IH".
+              iApply "H".
+              iPureIntro.
+              exists (RiscvPmpIrisHeapKit.pmp_permission p cfg).
+              unfold RiscvPmpIrisHeapKit.check_access,
+                RiscvPmpIrisHeapKit.pmp_check.
+              unfold In_entries in HIn.
+              simpl in HIn.
+              apply andb_true_iff in HIn as [Heq Ha].
+              apply Z.eqb_eq in Ha; subst.
+              apply pmpcfg_ent_eqb_iff in Heq as [= ->].
+              unfold Prev_addr in HPrev.
+              simpl in HPrev.
+              apply Z.eqb_eq in HPrev as [= ->].
+              rewrite (within_cfg_pmp_match_entry p HWithin); try assumption.
+
+              (* TODO: this will not scale well.. if more PMP entries are added,
+                     it would be better to have proof that it doesn't match
+                     preceding entries! *)
+              unfold RiscvPmpIrisHeapKit.pmp_match_entry,
+                RiscvPmpIrisHeapKit.pmp_match_addr,
+                RiscvPmpIrisHeapKit.pmp_addr_range.
+              destruct cfg0 as [? [] ? ? ?]; simpl; auto.
+              destruct (addr0 <? 0)%Z; auto.
+              unfold Within_cfg, decide_within_cfg in HWithin; simpl in HWithin.
+              destruct cfg1 as [? [] ? ? ?]; simpl in *; auto; try discriminate.
+              apply andb_leb_ltb_iff in HWithin as [H _].
+              rewrite ?Z.leb_antisym.
+              apply Z.ltb_ge in H as ->; simpl.
+              rewrite orb_true_r; auto.
+          + rewrite big_opL_cons.
+            iDestruct "Hpmp_addr_access" as "[_ H]".
+            iApply "IH"; try done.
+      }
+    Admitted.
+
   End Lemmas.
 
   Lemma lemSem `{sg : sailGS Σ} : LemmaSem (Σ := Σ).
   Proof.
     intros Δ [];
       eauto using open_gprs_sound, close_gprs_sound, open_pmp_entries_sound,
-      close_pmp_entries_sound.
-  Qed.
+      close_pmp_entries_sound, extract_pmp_ptsto_sound.
+  Admitted. (* TODO: back to Qed once the gen_addr_matching_cfg stuff is thrown away *)
 End RiscvPmpModel.
